Update OneHot2

Risc0/Gadgets/OneHot2/Constraints/CodeParts.lean
@@ -4,23 +4,40 @@ namespace Risc0.OneHot2.Constraints.Code
 
 open MLIRNotation
 
-def part0 : MLIRProgram :=   "%2" ←ₐ ⊤; "%0" ←ₐ .Const 0; "%3" ←ₐ .Get ⟨"code"⟩ 0 0; "%4" ←ₐ .Sub ⟨"%0"⟩ ⟨"%3"⟩
-def part1 : MLIRProgram :=   "%5" ←ₐ ⟨"%2"⟩ &₀ ⟨"%4"⟩; "%1" ←ₐ .Const 1; "%6" ←ₐ .Get ⟨"data"⟩ 0 0; "%7" ←ₐ .Sub ⟨"%1"⟩ ⟨"%6"⟩
-def part2 : MLIRProgram :=   "%8" ←ₐ .Mul ⟨"%6"⟩ ⟨"%7"⟩; "%9" ←ₐ ⟨"%5"⟩ &₀ ⟨"%8"⟩; "%10" ←ₐ .Sub ⟨"%6"⟩ ⟨"%1"⟩; "%11" ←ₐ ⟨"%9"⟩ &₀ ⟨"%10"⟩
+def part0 : MLIRProgram :=   "%1" ←ₐ ⊤; "%2" ←ₐ .Get ⟨"code"⟩ 0 0; "%3" ←ₐ .Get ⟨"data"⟩ 0 1; "%4" ←ₐ .Sub ⟨"%3"⟩ ⟨"%2"⟩
+def part1 : MLIRProgram :=   "%5" ←ₐ ⟨"%1"⟩ &₀ ⟨"%4"⟩; "%0" ←ₐ .Const 1; "%6" ←ₐ .Get ⟨"data"⟩ 0 0; "%7" ←ₐ .Sub ⟨"%0"⟩ ⟨"%6"⟩
+def part2 : MLIRProgram :=   "%8" ←ₐ .Mul ⟨"%6"⟩ ⟨"%7"⟩; "%9" ←ₐ ⟨"%5"⟩ &₀ ⟨"%8"⟩; "%10" ←ₐ .Sub ⟨"%0"⟩ ⟨"%3"⟩; "%11" ←ₐ .Mul ⟨"%3"⟩ ⟨"%10"⟩
+def part3 : MLIRProgram :=   "%12" ←ₐ ⟨"%9"⟩ &₀ ⟨"%11"⟩; "%13" ←ₐ .Add ⟨"%6"⟩ ⟨"%3"⟩; "%14" ←ₐ .Sub ⟨"%13"⟩ ⟨"%0"⟩; "%15" ←ₐ ⟨"%12"⟩ &₀ ⟨"%14"⟩
 
-def part0_to_end : MLIRProgram :=   "%2" ←ₐ ⊤; "%0" ←ₐ .Const 0; "%3" ←ₐ .Get ⟨"code"⟩ 0 0; "%4" ←ₐ .Sub ⟨"%0"⟩ ⟨"%3"⟩; "%5" ←ₐ ⟨"%2"⟩ &₀ ⟨"%4"⟩; "%1" ←ₐ .Const 1; "%6" ←ₐ .Get ⟨"data"⟩ 0 0; "%7" ←ₐ .Sub ⟨"%1"⟩ ⟨"%6"⟩; "%8" ←ₐ .Mul ⟨"%6"⟩ ⟨"%7"⟩; "%9" ←ₐ ⟨"%5"⟩ &₀ ⟨"%8"⟩; "%10" ←ₐ .Sub ⟨"%6"⟩ ⟨"%1"⟩; "%11" ←ₐ ⟨"%9"⟩ &₀ ⟨"%10"⟩
-def part1_to_end : MLIRProgram :=   "%5" ←ₐ ⟨"%2"⟩ &₀ ⟨"%4"⟩; "%1" ←ₐ .Const 1; "%6" ←ₐ .Get ⟨"data"⟩ 0 0; "%7" ←ₐ .Sub ⟨"%1"⟩ ⟨"%6"⟩; "%8" ←ₐ .Mul ⟨"%6"⟩ ⟨"%7"⟩; "%9" ←ₐ ⟨"%5"⟩ &₀ ⟨"%8"⟩; "%10" ←ₐ .Sub ⟨"%6"⟩ ⟨"%1"⟩; "%11" ←ₐ ⟨"%9"⟩ &₀ ⟨"%10"⟩
-def part2_to_end : MLIRProgram :=   "%8" ←ₐ .Mul ⟨"%6"⟩ ⟨"%7"⟩; "%9" ←ₐ ⟨"%5"⟩ &₀ ⟨"%8"⟩; "%10" ←ₐ .Sub ⟨"%6"⟩ ⟨"%1"⟩; "%11" ←ₐ ⟨"%9"⟩ &₀ ⟨"%10"⟩
+def part0_to_end : MLIRProgram :=   "%1" ←ₐ ⊤; "%2" ←ₐ .Get ⟨"code"⟩ 0 0; "%3" ←ₐ .Get ⟨"data"⟩ 0 1; "%4" ←ₐ .Sub ⟨"%3"⟩ ⟨"%2"⟩; "%5" ←ₐ ⟨"%1"⟩ &₀ ⟨"%4"⟩; "%0" ←ₐ .Const 1; "%6" ←ₐ .Get ⟨"data"⟩ 0 0; "%7" ←ₐ .Sub ⟨"%0"⟩ ⟨"%6"⟩; "%8" ←ₐ .Mul ⟨"%6"⟩ ⟨"%7"⟩; "%9" ←ₐ ⟨"%5"⟩ &₀ ⟨"%8"⟩; "%10" ←ₐ .Sub ⟨"%0"⟩ ⟨"%3"⟩; "%11" ←ₐ .Mul ⟨"%3"⟩ ⟨"%10"⟩; "%12" ←ₐ ⟨"%9"⟩ &₀ ⟨"%11"⟩; "%13" ←ₐ .Add ⟨"%6"⟩ ⟨"%3"⟩; "%14" ←ₐ .Sub ⟨"%13"⟩ ⟨"%0"⟩; "%15" ←ₐ ⟨"%12"⟩ &₀ ⟨"%14"⟩
+def part1_to_end : MLIRProgram :=   "%5" ←ₐ ⟨"%1"⟩ &₀ ⟨"%4"⟩; "%0" ←ₐ .Const 1; "%6" ←ₐ .Get ⟨"data"⟩ 0 0; "%7" ←ₐ .Sub ⟨"%0"⟩ ⟨"%6"⟩; "%8" ←ₐ .Mul ⟨"%6"⟩ ⟨"%7"⟩; "%9" ←ₐ ⟨"%5"⟩ &₀ ⟨"%8"⟩; "%10" ←ₐ .Sub ⟨"%0"⟩ ⟨"%3"⟩; "%11" ←ₐ .Mul ⟨"%3"⟩ ⟨"%10"⟩; "%12" ←ₐ ⟨"%9"⟩ &₀ ⟨"%11"⟩; "%13" ←ₐ .Add ⟨"%6"⟩ ⟨"%3"⟩; "%14" ←ₐ .Sub ⟨"%13"⟩ ⟨"%0"⟩; "%15" ←ₐ ⟨"%12"⟩ &₀ ⟨"%14"⟩
+def part2_to_end : MLIRProgram :=   "%8" ←ₐ .Mul ⟨"%6"⟩ ⟨"%7"⟩; "%9" ←ₐ ⟨"%5"⟩ &₀ ⟨"%8"⟩; "%10" ←ₐ .Sub ⟨"%0"⟩ ⟨"%3"⟩; "%11" ←ₐ .Mul ⟨"%3"⟩ ⟨"%10"⟩; "%12" ←ₐ ⟨"%9"⟩ &₀ ⟨"%11"⟩; "%13" ←ₐ .Add ⟨"%6"⟩ ⟨"%3"⟩; "%14" ←ₐ .Sub ⟨"%13"⟩ ⟨"%0"⟩; "%15" ←ₐ ⟨"%12"⟩ &₀ ⟨"%14"⟩
+def part3_to_end : MLIRProgram :=   "%12" ←ₐ ⟨"%9"⟩ &₀ ⟨"%11"⟩; "%13" ←ₐ .Add ⟨"%6"⟩ ⟨"%3"⟩; "%14" ←ₐ .Sub ⟨"%13"⟩ ⟨"%0"⟩; "%15" ←ₐ ⟨"%12"⟩ &₀ ⟨"%14"⟩
 
 abbrev parts_combined : MLIRProgram :=
-  part0; part1; part2
+  part0; part1; part2; part3
 
+lemma parts_combine3 :
+  Γ st ⟦part3⟧ =
+  Γ st ⟦part3_to_end⟧ := by
+    rfl
 lemma parts_combine2 :
-  Γ st ⟦part2⟧ =
+  Γ st ⟦part2; part3⟧ =
   Γ st ⟦part2_to_end⟧ := by
+    unfold part2
+    rewrite [MLIR.part_assoc_dddd]
+    apply MLIR.seq_step_eq
+    intro st
+    apply MLIR.seq_step_eq
+    intro st
+    apply MLIR.seq_step_eq
+    intro st
+    apply MLIR.seq_step_eq
+    intro st
+    rewrite [parts_combine3]
     rfl
 lemma parts_combine1 :
-  Γ st ⟦part1; part2⟧ =
+  Γ st ⟦part1; part2; part3⟧ =
   Γ st ⟦part1_to_end⟧ := by
     unfold part1
     rewrite [MLIR.part_assoc_dddd]
@@ -35,7 +52,7 @@ lemma parts_combine1 :
     rewrite [parts_combine2]
     rfl
 lemma parts_combine0 :
-  Γ st ⟦part0; part1; part2⟧ =
+  Γ st ⟦part0; part1; part2; part3⟧ =
   Γ st ⟦part0_to_end⟧ := by
     unfold part0
     rewrite [MLIR.part_assoc_dddd]
