Risc0/Gadgets/OneHot2/Constraints/CodeReordered.lean
@@ -8,41 +8,42 @@ namespace Risc0.OneHot2.Constraints.Code
 open MLIRNotation
 
 def opt1 : MLIRProgram :=
-  "%1" ←ₐ .Const 1; "%2" ←ₐ ⊤; "%3" ←ₐ .Get ⟨"code"⟩ 0 0; "%0" ←ₐ .Const 0; "%4" ←ₐ .Sub ⟨"%0"⟩ ⟨"%3"⟩; "%5" ←ₐ ⟨"%2"⟩ &₀ ⟨"%4"⟩; "%6" ←ₐ .Get ⟨"data"⟩ 0 0; "%7" ←ₐ .Sub ⟨"%1"⟩ ⟨"%6"⟩; "%8" ←ₐ .Mul ⟨"%6"⟩ ⟨"%7"⟩; "%9" ←ₐ ⟨"%5"⟩ &₀ ⟨"%8"⟩; "%10" ←ₐ .Sub ⟨"%6"⟩ ⟨"%1"⟩; "%11" ←ₐ ⟨"%9"⟩ &₀ ⟨"%10"⟩
+  "%1" ←ₐ ⊤; "%2" ←ₐ .Get ⟨"code"⟩ 0 0; "%3" ←ₐ .Get ⟨"data"⟩ 0 1; "%4" ←ₐ .Sub ⟨"%3"⟩ ⟨"%2"⟩; "%5" ←ₐ ⟨"%1"⟩ &₀ ⟨"%4"⟩; "%6" ←ₐ .Get ⟨"data"⟩ 0 0; "%0" ←ₐ .Const 1; "%7" ←ₐ .Sub ⟨"%0"⟩ ⟨"%6"⟩; "%8" ←ₐ .Mul ⟨"%6"⟩ ⟨"%7"⟩; "%9" ←ₐ ⟨"%5"⟩ &₀ ⟨"%8"⟩; "%10" ←ₐ .Sub ⟨"%0"⟩ ⟨"%3"⟩; "%11" ←ₐ .Mul ⟨"%3"⟩ ⟨"%10"⟩; "%12" ←ₐ ⟨"%9"⟩ &₀ ⟨"%11"⟩; "%13" ←ₐ .Add ⟨"%6"⟩ ⟨"%3"⟩; "%14" ←ₐ .Sub ⟨"%13"⟩ ⟨"%0"⟩; "%15" ←ₐ ⟨"%12"⟩ &₀ ⟨"%14"⟩
 lemma optimised_behaviour1 :
   getReturn (full.runProgram st)  =
   getReturn (opt1.runProgram st)  := by
     unfold getReturn MLIR.runProgram full
-    rewrite[opt_swap (const_past_const (by trivial)),opt_swap (const_past_true (by trivial)),opt_swap (const_past_get (by trivial))]
+    rewrite[opt_swap (const_past_true (by trivial)),opt_swap (const_past_get (by trivial)),opt_swap (const_past_get (by trivial)),opt_swap (const_past_sub (by trivial) (by trivial) (by trivial)),opt_swap (const_past_andEqz (by trivial)),opt_swap (const_past_get (by trivial))]
     simp only [←MLIR.run_nondet]
     rewrite [←MLIR.run_seq_def]
-    rewrite[←MLIR.run_seq_def,←MLIR.run_seq_def]
+    rewrite[←MLIR.run_seq_def,←MLIR.run_seq_def,←MLIR.run_seq_def,←MLIR.run_seq_def,←MLIR.run_seq_def]
     unfold opt1
     simp only
 
 def opt2 : MLIRProgram :=
-  "%2" ←ₐ ⊤; "%3" ←ₐ .Get ⟨"code"⟩ 0 0; "%0" ←ₐ .Const 0; "%4" ←ₐ .Sub ⟨"%0"⟩ ⟨"%3"⟩; "%5" ←ₐ ⟨"%2"⟩ &₀ ⟨"%4"⟩; "%6" ←ₐ .Get ⟨"data"⟩ 0 0; "%1" ←ₐ .Const 1; "%7" ←ₐ .Sub ⟨"%1"⟩ ⟨"%6"⟩; "%8" ←ₐ .Mul ⟨"%6"⟩ ⟨"%7"⟩; "%9" ←ₐ ⟨"%5"⟩ &₀ ⟨"%8"⟩; "%10" ←ₐ .Sub ⟨"%6"⟩ ⟨"%1"⟩; "%11" ←ₐ ⟨"%9"⟩ &₀ ⟨"%10"⟩
+  "%1" ←ₐ ⊤; "%3" ←ₐ .Get ⟨"data"⟩ 0 1; "%2" ←ₐ .Get ⟨"code"⟩ 0 0; "%4" ←ₐ .Sub ⟨"%3"⟩ ⟨"%2"⟩; "%5" ←ₐ ⟨"%1"⟩ &₀ ⟨"%4"⟩; "%6" ←ₐ .Get ⟨"data"⟩ 0 0; "%0" ←ₐ .Const 1; "%7" ←ₐ .Sub ⟨"%0"⟩ ⟨"%6"⟩; "%8" ←ₐ .Mul ⟨"%6"⟩ ⟨"%7"⟩; "%9" ←ₐ ⟨"%5"⟩ &₀ ⟨"%8"⟩; "%10" ←ₐ .Sub ⟨"%0"⟩ ⟨"%3"⟩; "%11" ←ₐ .Mul ⟨"%3"⟩ ⟨"%10"⟩; "%12" ←ₐ ⟨"%9"⟩ &₀ ⟨"%11"⟩; "%13" ←ₐ .Add ⟨"%6"⟩ ⟨"%3"⟩; "%14" ←ₐ .Sub ⟨"%13"⟩ ⟨"%0"⟩; "%15" ←ₐ ⟨"%12"⟩ &₀ ⟨"%14"⟩
 lemma optimised_behaviour2 :
   getReturn (full.runProgram st)  =
   getReturn (opt2.runProgram st)  := by
     rewrite [optimised_behaviour1]
     unfold getReturn MLIR.runProgram opt1
-    rewrite[opt_swap (const_past_true (by trivial)),opt_swap (const_past_get (by trivial)),opt_swap (const_past_const (by trivial)),opt_swap (const_past_sub (by trivial) (by trivial) (by trivial)),opt_swap (const_past_andEqz (by trivial)),opt_swap (const_past_get (by trivial))]
+    rewrite[MLIR.run_seq_def]
+    rewrite[opt_swap (get_past_get_buf (by trivial) (by trivial))]
     simp only [←MLIR.run_nondet]
     rewrite [←MLIR.run_seq_def]
-    rewrite[←MLIR.run_seq_def,←MLIR.run_seq_def,←MLIR.run_seq_def,←MLIR.run_seq_def,←MLIR.run_seq_def]
+    rewrite[←MLIR.run_seq_def]
     unfold opt2
     simp only
 
 def opt3 : MLIRProgram :=
-  "%2" ←ₐ ⊤; "%0" ←ₐ .Const 0; "%3" ←ₐ .Get ⟨"code"⟩ 0 0; "%4" ←ₐ .Sub ⟨"%0"⟩ ⟨"%3"⟩; "%5" ←ₐ ⟨"%2"⟩ &₀ ⟨"%4"⟩; "%6" ←ₐ .Get ⟨"data"⟩ 0 0; "%1" ←ₐ .Const 1; "%7" ←ₐ .Sub ⟨"%1"⟩ ⟨"%6"⟩; "%8" ←ₐ .Mul ⟨"%6"⟩ ⟨"%7"⟩; "%9" ←ₐ ⟨"%5"⟩ &₀ ⟨"%8"⟩; "%10" ←ₐ .Sub ⟨"%6"⟩ ⟨"%1"⟩; "%11" ←ₐ ⟨"%9"⟩ &₀ ⟨"%10"⟩
+  "%1" ←ₐ ⊤; "%2" ←ₐ .Get ⟨"code"⟩ 0 0; "%3" ←ₐ .Get ⟨"data"⟩ 0 1; "%4" ←ₐ .Sub ⟨"%3"⟩ ⟨"%2"⟩; "%5" ←ₐ ⟨"%1"⟩ &₀ ⟨"%4"⟩; "%6" ←ₐ .Get ⟨"data"⟩ 0 0; "%0" ←ₐ .Const 1; "%7" ←ₐ .Sub ⟨"%0"⟩ ⟨"%6"⟩; "%8" ←ₐ .Mul ⟨"%6"⟩ ⟨"%7"⟩; "%9" ←ₐ ⟨"%5"⟩ &₀ ⟨"%8"⟩; "%10" ←ₐ .Sub ⟨"%0"⟩ ⟨"%3"⟩; "%11" ←ₐ .Mul ⟨"%3"⟩ ⟨"%10"⟩; "%12" ←ₐ ⟨"%9"⟩ &₀ ⟨"%11"⟩; "%13" ←ₐ .Add ⟨"%6"⟩ ⟨"%3"⟩; "%14" ←ₐ .Sub ⟨"%13"⟩ ⟨"%0"⟩; "%15" ←ₐ ⟨"%12"⟩ &₀ ⟨"%14"⟩
 lemma optimised_behaviour3 :
   getReturn (full.runProgram st)  =
   getReturn (opt3.runProgram st)  := by
     rewrite [optimised_behaviour2]
     unfold getReturn MLIR.runProgram opt2
     rewrite[MLIR.run_seq_def]
-    rewrite[opt_swap (get_past_const (by trivial))]
+    rewrite[opt_swap (get_past_get_buf (by trivial) (by trivial))]
     simp only [←MLIR.run_nondet]
     rewrite [←MLIR.run_seq_def]
     rewrite[←MLIR.run_seq_def]
@@ -50,7 +51,7 @@ lemma optimised_behaviour3 :
     simp only
 
 def opt4 : MLIRProgram :=
-  "%2" ←ₐ ⊤; "%0" ←ₐ .Const 0; "%3" ←ₐ .Get ⟨"code"⟩ 0 0; "%4" ←ₐ .Sub ⟨"%0"⟩ ⟨"%3"⟩; "%5" ←ₐ ⟨"%2"⟩ &₀ ⟨"%4"⟩; "%1" ←ₐ .Const 1; "%6" ←ₐ .Get ⟨"data"⟩ 0 0; "%7" ←ₐ .Sub ⟨"%1"⟩ ⟨"%6"⟩; "%8" ←ₐ .Mul ⟨"%6"⟩ ⟨"%7"⟩; "%9" ←ₐ ⟨"%5"⟩ &₀ ⟨"%8"⟩; "%10" ←ₐ .Sub ⟨"%6"⟩ ⟨"%1"⟩; "%11" ←ₐ ⟨"%9"⟩ &₀ ⟨"%10"⟩
+  "%1" ←ₐ ⊤; "%2" ←ₐ .Get ⟨"code"⟩ 0 0; "%3" ←ₐ .Get ⟨"data"⟩ 0 1; "%4" ←ₐ .Sub ⟨"%3"⟩ ⟨"%2"⟩; "%5" ←ₐ ⟨"%1"⟩ &₀ ⟨"%4"⟩; "%0" ←ₐ .Const 1; "%6" ←ₐ .Get ⟨"data"⟩ 0 0; "%7" ←ₐ .Sub ⟨"%0"⟩ ⟨"%6"⟩; "%8" ←ₐ .Mul ⟨"%6"⟩ ⟨"%7"⟩; "%9" ←ₐ ⟨"%5"⟩ &₀ ⟨"%8"⟩; "%10" ←ₐ .Sub ⟨"%0"⟩ ⟨"%3"⟩; "%11" ←ₐ .Mul ⟨"%3"⟩ ⟨"%10"⟩; "%12" ←ₐ ⟨"%9"⟩ &₀ ⟨"%11"⟩; "%13" ←ₐ .Add ⟨"%6"⟩ ⟨"%3"⟩; "%14" ←ₐ .Sub ⟨"%13"⟩ ⟨"%0"⟩; "%15" ←ₐ ⟨"%12"⟩ &₀ ⟨"%14"⟩
 lemma optimised_behaviour4 :
   getReturn (full.runProgram st)  =
   getReturn (opt4.runProgram st)  := by
