Risc0/Gadgets/OneHot2/Constraints/WeakestPresPart2.lean
@@ -18,32 +18,29 @@ def part2_state (st: State) : State :=
                 (Option.get! (State.felts st { name := "%6" : FeltVar }) = (0 : Felt) ∨
                   Option.get! (State.felts st { name := "%7" : FeltVar }) =
                     (0 : Felt))))[felts][{ name := "%10" : FeltVar }] ←
-            Option.get! (State.felts st { name := "%6" : FeltVar }) -
-              Option.get! (State.felts st { name := "%1" : FeltVar }))[props][{ name := "%11" : PropVar }] ←
-          ((Option.get! (State.props st { name := "%5" : PropVar }) ∧
-              (Option.get! (State.felts st { name := "%6" : FeltVar }) = (0 : Felt) ∨
-                Option.get! (State.felts st { name := "%7" : FeltVar }) = (0 : Felt))) ∧
-            Option.get! (State.felts st { name := "%6" : FeltVar }) -
-                Option.get! (State.felts st { name := "%1" : FeltVar }) =
-              (0 : Felt))) 
+            Option.get! (State.felts st { name := "%0" : FeltVar }) -
+              Option.get! (State.felts st { name := "%3" : FeltVar }))[felts][{ name := "%11" : FeltVar }] ←
+          Option.get! (State.felts st { name := "%3" : FeltVar }) *
+            (Option.get! (State.felts st { name := "%0" : FeltVar }) -
+              Option.get! (State.felts st { name := "%3" : FeltVar }))) 
 
 def part2_drops (st: State) : State :=
-  State.dropFelts (State.dropFelts (State.dropFelts (State.dropFelts (State.dropFelts (st) ⟨"%1"⟩) ⟨"%6"⟩) ⟨"%7"⟩) ⟨"%8"⟩) ⟨"%10"⟩
+  State.dropFelts (State.dropFelts (State.dropFelts (st) ⟨"%7"⟩) ⟨"%8"⟩) ⟨"%10"⟩
 
 -- Run the program from part2 onwards by using part2_state rather than Code.part2
 def part2_state_update (st: State): State :=
-  part2_drops (part2_state st)
+  Γ (part2_drops (part2_state st)) ⟦Code.part3;dropfelt ⟨"%3"⟩;dropfelt ⟨"%0"⟩;dropfelt ⟨"%6"⟩;dropfelt ⟨"%11"⟩;dropfelt ⟨"%13"⟩;dropfelt ⟨"%14"⟩⟧
 
 -- Prove that substituting part2_state for Code.part2 produces the same result
-lemma part2_wp {st : State}:
-  Code.getReturn (MLIR.runProgram (Code.part2;dropfelt ⟨"%1"⟩;dropfelt ⟨"%6"⟩;dropfelt ⟨"%7"⟩;dropfelt ⟨"%8"⟩;dropfelt ⟨"%10"⟩) st) ↔
+lemma part2_wp {st : State} :
+  Code.getReturn (MLIR.runProgram (Code.part2;dropfelt ⟨"%7"⟩;dropfelt ⟨"%8"⟩;dropfelt ⟨"%10"⟩;Code.part3;dropfelt ⟨"%3"⟩;dropfelt ⟨"%0"⟩;dropfelt ⟨"%6"⟩;dropfelt ⟨"%11"⟩;dropfelt ⟨"%13"⟩;dropfelt ⟨"%14"⟩) st) ↔
   Code.getReturn (part2_state_update st) := by
   unfold MLIR.runProgram; simp only
-  generalize eq : (dropfelt ⟨"%1"⟩;dropfelt ⟨"%6"⟩;dropfelt ⟨"%7"⟩;dropfelt ⟨"%8"⟩;dropfelt ⟨"%10"⟩) = prog
+  generalize eq : (dropfelt ⟨"%7"⟩;dropfelt ⟨"%8"⟩;dropfelt ⟨"%10"⟩;Code.part3;dropfelt ⟨"%3"⟩;dropfelt ⟨"%0"⟩;dropfelt ⟨"%6"⟩;dropfelt ⟨"%11"⟩;dropfelt ⟨"%13"⟩;dropfelt ⟨"%14"⟩) = prog
   unfold Code.part2
   MLIR
   rewrite [←eq]
-  rewrite [MLIR.run_seq_def,MLIR.run_dropfelt, MLIR.run_seq_def,MLIR.run_dropfelt, MLIR.run_seq_def,MLIR.run_dropfelt, MLIR.run_seq_def,MLIR.run_dropfelt, MLIR.run_dropfelt]
+  rewrite [MLIR.run_seq_def,MLIR.run_dropfelt, MLIR.run_seq_def,MLIR.run_dropfelt, MLIR.run_seq_def,MLIR.run_dropfelt]
   unfold part2_state_update part2_drops part2_state
   rfl
 
@@ -56,21 +53,22 @@ lemma part2_cumulative_wp {code0 data0 data1: Felt} :
   Code.run (start_state ([code0]) ([data0, data1])) ↔
   Code.getReturn
       (part2_state_update
-        ((((({
-                    buffers :=
-                      ((fun x => Map.empty x)[{ name := "data" : BufferVar }] ←ₘ
-                          [[some data0, some data1]])[{ name := "code" : BufferVar }] ←ₘ
-                        [[some code0]],
-                    bufferWidths :=
-                      ((fun x => Map.empty x)[{ name := "data" : BufferVar }] ←ₘ
-                          (2 : ℕ))[{ name := "code" : BufferVar }] ←ₘ
-                        (1 : ℕ),
-                    constraints := [], cycle := (0 : ℕ), felts := Map.empty, isFailed := false, props := Map.empty,
-                    vars :=
-                      [{ name := "code" : BufferVar },
-                        { name := "data" : BufferVar }] }[props][{ name := "%2" : PropVar }] ←
-                  True)[props][{ name := "%5" : PropVar }] ←
-                code0 = (0 : Felt))[felts][{ name := "%1" : FeltVar }] ←
+        (((((({
+                      buffers :=
+                        ((fun x => Map.empty x)[{ name := "data" : BufferVar }] ←ₘ
+                            [[some data0, some data1]])[{ name := "code" : BufferVar }] ←ₘ
+                          [[some code0]],
+                      bufferWidths :=
+                        ((fun x => Map.empty x)[{ name := "data" : BufferVar }] ←ₘ
+                            (2 : ℕ))[{ name := "code" : BufferVar }] ←ₘ
+                          (1 : ℕ),
+                      constraints := [], cycle := (0 : ℕ), felts := Map.empty, isFailed := false, props := Map.empty,
+                      vars :=
+                        [{ name := "code" : BufferVar },
+                          { name := "data" : BufferVar }] }[props][{ name := "%1" : PropVar }] ←
+                    True)[felts][{ name := "%3" : FeltVar }] ←
+                  data1)[props][{ name := "%5" : PropVar }] ←
+                data1 - code0 = (0 : Felt))[felts][{ name := "%0" : FeltVar }] ←
               (1 : Felt))[felts][{ name := "%6" : FeltVar }] ←
             data0)[felts][{ name := "%7" : FeltVar }] ←
           (1 : Felt) - data0))  := by
@@ -90,31 +88,7 @@ lemma part2_cumulative_wp {code0 data0 data1: Felt} :
     -- 0 sets
     -- rewrite [Map.drop_of_updates]
     -- simp only [Map.drop_base, ne_eq, Map.update_drop_swap, Map.update_drop]
-    -- there are statements after an if
-    try simp [State.buffers_if_eq_if_buffers,State.bufferWidths_if_eq_if_bufferWidths,State.constraints_if_eq_if_constraints,State.cycle_if_eq_if_cycle,State.felts_if_eq_if_felts,State.isFailed_if_eq_if_isFailed,State.props_if_eq_if_props,State.vars_if_eq_if_vars]
+    -- there are not any statements after an if
+    -- try simp [State.buffers_if_eq_if_buffers,State.bufferWidths_if_eq_if_bufferWidths,State.constraints_if_eq_if_constraints,State.cycle_if_eq_if_cycle,State.felts_if_eq_if_felts,State.isFailed_if_eq_if_isFailed,State.props_if_eq_if_props,State.vars_if_eq_if_vars]
 
-lemma closed_form {code0 data0 data1: Felt} :
-  Code.run (start_state ([code0]) ([data0, data1])) ↔
-   (code0 = (0 : Felt) ∧ (data0 = (0 : Felt) ∨ (1 : Felt) - data0 = (0 : Felt))) ∧ data0 - (1 : Felt) = (0 : Felt)  := by
-    rewrite [part2_cumulative_wp]
-    unfold part2_state_update
-    unfold part2_state
-    MLIR_states_updates
-    -- 0 withEqZeros
-    -- rewrite [withEqZero_def]
-    -- MLIR_states_updates
-    unfold part2_drops
-    -- 5 drops
-    simp only [State.drop_update_swap, State.drop_update_same, State.drop_updateProps_swap]
-    rewrite [State.dropFelts]
-    simp only [State.dropFelts_buffers, State.dropFelts_bufferWidths, State.dropFelts_constraints, State.dropFelts_cycle, State.dropFelts_felts, State.dropFelts_isFailed, State.dropFelts_props, State.dropFelts_vars]
-    simp only [Map.drop_base, ne_eq, Map.update_drop_swap, Map.update_drop]
-    -- 0 sets
-    -- rewrite [Map.drop_of_updates]
-    -- simp only [Map.drop_base, ne_eq, Map.update_drop_swap, Map.update_drop]
-    -- there are statements after an if
-    try simp [State.buffers_if_eq_if_buffers,State.bufferWidths_if_eq_if_bufferWidths,State.constraints_if_eq_if_constraints,State.cycle_if_eq_if_cycle,State.felts_if_eq_if_felts,State.isFailed_if_eq_if_isFailed,State.props_if_eq_if_props,State.vars_if_eq_if_vars]
-    unfold Code.getReturn
-    simp only
-    simp only [Code.getReturn, State.constraintsInVar, State.updateProps_props_get_wobbly, Option.getD_some]
 end Risc0.OneHot2.Constraints.WP
